# Untersuchung der Frage

Hier soll die Aussage
$$abcd+bcda = ab\wedge c\wedge d + b\wedge c\wedge da$$
untersucht werden.
$$\begin{align*}
  abcd &= a(bcd) \\
  &= a(b\cdot cd + b\wedge cd) \\
  &= b\cdot cad + ab\wedge cd \\
  &= b\cdot ca\cdot d + b\cdot ca\wedge d +ab\wedge cd \\
  &= b\cdot ca\cdot d + b\cdot ca\wedge d +a(b\wedge c\cdot d + b\wedge c\wedge
  d)
\end{align*}$$
$$\begin{align*}
  bcda &= (bcd)a \\
  &= (b\cdot cd + b\wedge cd)a \\
  &= b\cdot cda + b\wedge cda \\
  &= b\cdot cd\cdot a + b\cdot cd\wedge a +b\wedge cda \\
  &= b\cdot cd\cdot a + b\cdot cd\wedge a +(b\wedge c\cdot d + b\wedge c\wedge
  d)a
\end{align*}$$
Nebenrechnung
$$\begin{align*}
  a(b\wedge c\cdot d) &= a(c\cdot db - b\cdot dc) \\
  &= c\cdot dab - b\cdot dac
\end{align*}$$
$$\begin{align*}
  (b\wedge c\cdot d)a &= (c\cdot db - b\cdot dc)a \\
  &= c\cdot dba - b\cdot dca
\end{align*}$$
Zeiter Ansatz
$$\begin{align*}
  bcda &= (bcd)a \\
  &= (bc\cdot d + bc\wedge d)a \\
  &= bac\cdot d + bc\wedge da \\
  &= b\cdot ac\cdot d + b\wedge ac\cdot d + bc\wedge da \\
  &= b\cdot ac\cdot d + b\wedge ac\cdot d + (b\cdot c\wedge d + b\wedge c\wedge
  d)a
\end{align*}$$

## Referenzen
- [Geometrische Algebra](f35d.md)
- [Herleitung f√ºr 3-Blades](3k2f.md)
